theories/Simple/DBToPIR.v
@@ -1,0 +1,278 @@
+From Coq Require Import Strings.String List Nat.
+Import ListNotations.
+
+From VTL Require Export PIR BigStepPIR Utils.
+
+(* More difficult translation from a nameless STLC that uses De Bruijn
+indices and a context to PIR, similar to the main proof as λ□ is also nameless *)
+
+Inductive ty : Type :=
+  | Ty_Bool  : ty
+  | Ty_Arrow : ty -> ty -> ty
+  | Ty_ERROR : ty.
+
+Inductive tm : Type :=
+  | tm_rel   : nat -> tm
+  | tm_app   : tm -> tm -> tm
+  | tm_abs   : string -> ty -> tm -> tm
+  | tm_true  : tm
+  | tm_false : tm
+  | tm_oops  : tm.
+
+Inductive translatesTypeTo : ty -> PIR.ty -> Prop :=
+  | tlty_bool  : translatesTypeTo Ty_Bool (PIR.Ty_Builtin DefaultUniBool)
+  | tlty_arrow : forall ty1 ty2 ty1' ty2',
+      translatesTypeTo ty1 ty1' ->
+      translatesTypeTo ty2 ty2' ->
+      translatesTypeTo (Ty_Arrow ty1 ty2) (PIR.Ty_Fun ty1' ty2').
+
+From MetaCoq.Utils Require Import utils.
+Import MCMonadNotation.
+
+Import Strings.String Nat.
+Local Open Scope string_scope.
+
+(* fresh variable generation *)
+Fixpoint gen_fresh_aux x (Γ : list string) n :=
+  match n with
+  | 0 => x
+  | S n' => let x' := x ++ "'" in 
+      if existsb (Strings.String.eqb x') Γ then gen_fresh_aux x' Γ n' else x'
+  end.
+
+Definition gen_fresh x (Γ : list string) :=
+  gen_fresh_aux x Γ #|Γ|.
+
+Lemma gen_fresh_fresh x (Γ : list string) :
+  ~ (In (gen_fresh x Γ) Γ).
+Proof.
+  unfold gen_fresh.
+Admitted.
+
+(* substitution *)
+Fixpoint lift n k nt : tm :=
+  match nt with
+  | tm_rel i => if Nat.leb k i then tm_rel (n + i) else tm_rel i
+  | tm_app t1 t2 => tm_app (lift n k t1) (lift n k t2)
+  | tm_abs x T b => tm_abs x T (lift n (S k) b)
+  | tm_true => tm_true
+  | tm_false => tm_false
+  | tm_oops => tm_oops end.
+
+Notation lift0 n := (lift n 0).
+Definition up := lift 1 0.
+
+Fixpoint closedn k nt : bool :=
+  match nt with
+  | tm_rel i => Nat.ltb i k 
+  | tm_app t1 t2 => closedn k t1 && closedn k t2
+  | tm_abs x T b => closedn (S k) b
+  | tm_oops => false
+  | _ => true end.
+
+Notation closed t := (closedn 0 t).
+
+Fixpoint csubst k s t : tm :=
+  match t with
+  | tm_rel n => if (k =? n)%nat then s else tm_rel n
+  | tm_app t1 t2 => tm_app (csubst k s t1) (csubst k s t2)
+  | tm_abs x T b => tm_abs x T (csubst (S k) s b)
+  | tm_true => tm_true
+  | tm_false => tm_false
+  | tm_oops => tm_oops end.
+
+Lemma csubst_closed k v t : closedn k t -> csubst k v t = t.
+Proof.
+  revert k. induction t; intros k' Hcl; inversion Hcl.
+  - apply ltb_lt, lt_neq, neq_sym, eqb_neq in H0.
+    simpl. rewrite H0. reflexivity.
+  - apply andb_true_iff in H0 as [Hcl1 Hcl2]. simpl.
+    rewrite (IHt1 k' Hcl1), (IHt2 k' Hcl2). reflexivity.
+  - simpl. rewrite (IHt (S k') H0). reflexivity.
+  - reflexivity.
+  - reflexivity.
+Qed.
+
+Inductive eval : tm -> tm -> Prop :=
+  | EN_Abs : forall x T b,
+      eval (tm_abs x T b) (tm_abs x T b)
+  | EN_App : forall t1 t2 x ty b v2 v,
+      eval t1 (tm_abs x ty b) ->
+      eval t2 v2 ->
+      eval (csubst 0 v2 b) v ->
+      eval (tm_app t1 t2) v
+  | EN_True  : eval tm_true tm_true
+  | EN_False : eval tm_false tm_false.
+
+Inductive translatesTo (Γ : list string) : tm -> term -> Prop :=
+  | tlt_rel : forall n x, 
+      find_index Γ x = Some n -> 
+      translatesTo Γ (tm_rel n) (Var x)
+  | tlt_abs : forall x x' ty ty' b b',
+      translatesTypeTo ty ty' ->
+      translatesTo (x' :: Γ) b b' ->
+      translatesTo Γ (tm_abs x ty b) (LamAbs x' ty' b')
+  | tlt_app : forall t1 t2 t1' t2',
+      translatesTo Γ t1 t1' ->
+      translatesTo Γ t2 t2' ->
+      translatesTo Γ (tm_app t1 t2) (Apply t1' t2')
+  | tlt_true : translatesTo Γ tm_true (Constant (ValueOf DefaultUniBool true))
+  | tlt_false : translatesTo Γ tm_false (Constant (ValueOf DefaultUniBool false)).
+
+Lemma weaken_ctx : forall Γ x t t',
+  translatesTo Γ t t' ->
+  translatesTo (Γ ++ [x]) t t'.
+Proof.
+  intros Γ' x' t. revert Γ' x'.
+  induction t; intros Γ x t' tlt_t;
+  inversion tlt_t; subst.
+  - apply tlt_rel. now apply find_index_weaken.
+  - apply tlt_app. 
+    apply IHt1. apply H1.
+    apply IHt2. apply H3.
+  - specialize (IHt (x' :: Γ) x b' H4).
+    apply tlt_abs; assumption.
+  - apply tlt_true.
+  - apply tlt_false.
+Qed.
+
+Lemma weaken_ctx_many : forall Γ1 Γ2 t t',
+  translatesTo Γ1 t t' ->
+  translatesTo (Γ1 ++ Γ2) t t'.
+Proof.
+  intros Γ1 Γ2 t. revert Γ1. induction t;
+  intros Γ1 t' tlt_t; inversion tlt_t; subst.
+  - apply tlt_rel. now apply find_index_weaken.
+  - apply tlt_app.
+    apply IHt1; assumption.
+    apply IHt2; assumption.
+  - apply tlt_abs. assumption.
+    now apply (IHt (x' :: Γ1)). 
+  - apply tlt_true.
+  - apply tlt_false.
+Qed.
+
+Lemma csubst_shadowed : forall Γ x b b' v,
+  In x Γ ->
+  translatesTo (Γ ++ [x]) b b' ->
+  csubst (List.length Γ) v b = b.
+Proof.
+  intros Γ x b. revert Γ. induction b; 
+  intros Γ b' v Hin tlt; inversion tlt.
+  - simpl.
+    destruct_nat_eq (List.length Γ) n.
+    + subst. apply find_index_outer in H0 as Hx.
+      subst x. now apply find_index_outer_not_In in H0.
+    + reflexivity.
+  - simpl.
+    rewrite (IHb1 Γ t1' v); try assumption.
+    rewrite (IHb2 Γ t2' v); try assumption.
+    reflexivity.
+  - specialize (IHb (x' :: Γ) b'0 v).
+    simpl in *. rewrite IHb; auto.
+  - reflexivity.
+  - reflexivity.
+Qed.
+
+Lemma strengthen_shadowed_ctx : forall Γ x b b',
+  In x Γ ->
+  translatesTo (Γ ++ [x]) b b' ->
+  translatesTo Γ b b'.
+Proof.
+  intros Γ x b. revert Γ. induction b;
+  intros Γ b' Hin tlt; inversion tlt; subst.
+  - apply tlt_rel. 
+    destruct_str_eq x x0.
+    + subst. now rewrite find_index_app1 in H0.
+    + rewrite find_index_app1 in H0. auto.
+      now eapply find_index_not_outer.
+  - apply tlt_app.
+    apply IHb1; assumption.
+    apply IHb2; assumption.
+  - apply tlt_abs. assumption.
+    apply IHb. now right. assumption.
+  - apply tlt_true.
+  - apply tlt_false.
+Qed.
+
+Lemma csubst_correct : forall Γ x v b v' b',
+  ~ In x Γ ->
+  translatesTo nil v v' ->
+  translatesTo (Γ ++ [x]) b b' ->
+  translatesTo Γ (csubst (List.length Γ) v b) (BigStepPIR.subst x v' b').
+Proof.
+  intros Γ x v b. revert Γ. induction b;
+  intros Γ v' b' HnIn tlt_v tlt_b;
+  inversion tlt_b.
+  - subst. simpl. destruct_str_eq x x0.
+    + subst. apply find_index_outer_length in H0 as Hl; auto.
+      symmetry in Hl. apply eqb_eq in Hl. rewrite Hl.
+      now eapply weaken_ctx_many in tlt_v.
+    + apply find_index_not_outer in H0 as Hin; auto.
+      apply find_index_not_outer_length in H0 as Hl; auto.
+      rewrite find_index_app1 in H0; auto. rewrite Hl.
+      now apply tlt_rel.
+  - simpl. apply tlt_app.
+    apply IHb1; assumption.
+    apply IHb2; assumption.
+  - subst. simpl. destruct_str_eq x x'.
+    + subst x'. apply tlt_abs. assumption.
+      assert (Hin : In x (x::Γ)). now left.
+      specialize (strengthen_shadowed_ctx (x :: Γ) x b b'0 Hin H4) as Hctx.
+      specialize (csubst_shadowed (x :: Γ) x b b'0 v Hin H4) as H1.
+      simpl in H1. now rewrite H1.
+    + apply tlt_abs; try assumption.
+      apply IHb; auto. now apply not_in_cons.
+  - apply tlt_true.
+  - apply tlt_false.
+Qed.
+
+Theorem translate_correct : forall t v t',
+  eval t v ->
+  translatesTo [] t t' ->
+  exists v' k,
+    translatesTo [] v v' /\
+    BigStepPIR.eval t' v' k.
+Proof with (eauto using BigStepPIR.eval).
+  intros t v t'' evn. revert t''; induction evn; 
+  intros t' tln_t; inversion tln_t.
+  - exists t'. eexists. subst...
+  - subst.
+    destruct (IHevn1 t1' H1) as [v1' [k1 [tlt_l ev_l]]].
+    destruct (IHevn2 t2' H3) as [v2' [k2 [nln_v2 ev_v2]]].
+    inversion tlt_l. subst.
+    assert (Hs : translatesTo [] (csubst 0 v2 b) (BigStepPIR.subst x' v2' b')).
+    apply (csubst_correct [] x' v2 b v2' b'); auto.
+    destruct (IHevn3 (BigStepPIR.subst x' v2' b') Hs) as [v' [k3 [tlt_s ev_s]]].
+    exists v'. eexists. split. apply tlt_s. eapply E_Apply. eexists.
+    apply ev_l. apply ev_v2. apply ev_s.
+  - exists t'. eexists. subst...
+  - exists t'. eexists. subst...
+Qed.
+
+Theorem allowed_shadowing Γ :
+  let nt := tm_abs "x" Ty_Bool 
+              (tm_abs "x" Ty_Bool (tm_rel 0)) in
+  let pt := LamAbs "x" (Ty_Builtin DefaultUniBool) 
+              (LamAbs "x" (Ty_Builtin DefaultUniBool) (Var "x")) in
+  translatesTo Γ nt pt.
+Proof.
+  intros. unfold nt, pt.
+  apply tlt_abs. apply tlty_bool.
+  apply tlt_abs. apply tlty_bool.
+  apply tlt_rel. apply find_index_first.
+Qed.
+
+Theorem disallowed_shadowing Γ n :
+  n > 0 ->
+  let nt := tm_abs "x" Ty_Bool 
+              (tm_abs "x" Ty_Bool (tm_rel n)) in
+  let pt := LamAbs "x" (Ty_Builtin DefaultUniBool) 
+              (LamAbs "x" (Ty_Builtin DefaultUniBool) (Var "x")) in
+  ~ translatesTo (Γ ++ ["x"]) nt pt.
+Proof.
+  unfold not. intros Hn tlt. 
+  invs tlt. invs H6. invs H8. 
+  apply find_index_Some_first in H3. 
+  apply lt_neq, neq_sym in Hn. contradiction. 
+Qed.
