theories/Simple/SimplePipeline.v
@@ -1,0 +1,48 @@
+From Coq Require Import Program.
+From MetaCoq.Utils Require Import utils.
+From MetaCoq.Common Require Import Transform config.
+
+From VTL.Simple Require Import DBToPIR.
+From VTL.Semantics Require Import BigStepPIR.
+
+(* A end-to-end pipeline from Coq/Gallina terms to PIR terms (with bogus types):
+   Gallina ▷ PCUIC ▷ λ□/EAst (without box type annotations) ▷ DB ▷ PIR *)
+
+Import Common.Transform.Transform.
+#[local] Obligation Tactic := program_simpl.
+
+Definition default_pir_fuel := 5000.
+
+Definition tm_program  := unit × tm.
+Definition pir_program := unit × term.
+
+Definition eval_tm_program  (p : tm_program)  (v  : tm)   := ∥ DBToPIR.eval p.2 v ∥.
+Definition eval_pir_program (p : pir_program) (v' : term) := ∥ BigStepPIR.eval p.2 v' default_pir_fuel ∥.
+
+Axiom translate_named : tm -> term.
+Definition translate_named_program (p : tm_program) := (tt, translate_named p.2).
+
+Program Definition stlc_to_pir_transform :
+  Transform.t unit unit tm term tm term
+  eval_tm_program
+  eval_pir_program :=
+  {| name := "translate stlc to pir terms";
+     transform input _ := _;
+     obseq p _ p' v v' := translatesTo [] v v' ;
+  |}.
+Next Obligation.
+(* pre? *) exact True.
+Qed.
+Next Obligation.
+(* pre is true of input *) Admitted.
+Next Obligation.
+(* post *) exact True.
+Qed.
+Next Obligation.
+(* pre establishes post *)
+Admitted.
+Next Obligation.
+  (* exact (translate_correct p.2 v p'.2 (∥ evalNamed p.2 v ∥) (∥ eval p'.2 v'∥)). *)
+Admitted.
+
+Check run stlc_to_pir_transform.
